WIP: manual heap: structured addresses

ulib/FStar.ManualST.fst
@@ -33,26 +33,45 @@ let gst_wp (a:Type)   = st_wp_h heap a
 unfold let lift_div_gst (a:Type) (wp:pure_wp a) (p:gst_post a) (h:heap) = wp (fun a -> p a h)
 sub_effect DIV ~> GST = lift_div_gst
 
-let heap_rel (h1:heap) (h2:heap) =
-  forall (a:Type0) (rel:preorder a) (r:mref a rel).
-    (r `freed_in` h1 ==> r `freed_in` h2)
-  /\ (h1 `contains` r ==> (h2 `contains` r ==> sel h1 r `rel` sel h2 r))
-  /\ (h1 `contains` r ==> h2 `contains` r \/ r `freed_in` h2)
-  /\ (r `unused_in` h2 ==> r `unused_in` h1)
+open FStar.Monotonic.ManualHeap
+friend FStar.Monotonic.ManualHeap
 
-//assume val gst_get: unit    -> GST heap (fun p h0 -> p h0 h0)
-//assume val gst_put: h1:heap -> GST unit (fun p h0 -> heap_rel h0 h1 /\ p () h1)
+
+let heap_rel (h1:heap) (h2:heap) =
+  (forall (a:Type0) (rel:preorder a) (r:mref a rel).
+      (r `freed_in` h1 ==> r `freed_in` h2)
+    /\ (h1 `contains` r ==> (h2 `contains` r ==> sel h1 r `rel` sel h2 r))
+    /\ (h1 `contains` r ==> h2 `contains` r \/ r `freed_in` h2)
+    /\ (r `unused_in` h2 ==> r `unused_in` h1)) /\
+  prefix (pos_of h1) (pos_of h2) /\
+  frozen_on (pos_of h1) h1 h2
+
+assume val gst_get: unit    -> GST heap (fun p h0 -> p h0 h0)
+assume val gst_put: h1:heap -> GST unit (fun p h0 -> heap_rel h0 h1 /\ p () h1)
 
 type heap_predicate = heap -> Type0
 
 let stable (p:heap_predicate) =
   forall (h1:heap) (h2:heap). (p h1 /\ heap_rel h1 h2) ==> p h2
 
+#set-options "--log_queries --z3refresh"
+
+let test (h1 h2 h3 : heap) (_ : squash (heap_rel h1 h2)) (_ : squash (heap_rel h2 h3)) =
+  //assert (heap_rel h1 h1);
+  assert (heap_rel h1 h3);
+  ()
+
+let test2 (h1 h2 h3 : heap) (_ : (heap_rel h1 h2)) (_ : heap_rel h2 h3) =
+  assert (heap_rel h1 h2);
+  assert (heap_rel h2 h3);
+  assert (heap_rel h1 h3);
+  ()
+
 abstract let witnessed (p:heap_predicate{stable p}) :Type0 =
   W.witnessed heap_rel p
 
-//assume val gst_witness: p:heap_predicate -> GST unit (fun post h0 -> stable p /\ p h0 /\ (witnessed p ==> post () h0))
-//assume val gst_recall:  p:heap_predicate -> GST unit (fun post h0 -> stable p /\ witnessed p /\ (p h0 ==> post () h0))
+private assume val gst_witness: p:heap_predicate -> GST unit (fun post h0 -> stable p /\ p h0 /\ (witnessed p ==> post () h0))
+private assume val gst_recall:  p:heap_predicate -> GST unit (fun post h0 -> stable p /\ witnessed p /\ (p h0 ==> post () h0))
 
 val lemma_functoriality (p:heap_predicate{stable p /\ witnessed p}) 
                         (q:heap_predicate{stable q /\ (forall (h:heap). p h ==> q h)})
@@ -77,7 +96,6 @@ effect ST (a:Type) (pre:st_pre) (post: (h:heap -> Tot (st_post' a (pre h)))) =
   STATE a (fun (p:st_post a) (h:heap) -> pre h /\ (forall a h1. post h a h1 ==> p a h1))
 effect St (a:Type) = ST a (fun h -> True) (fun h0 r h1 -> True)
 
-
 let stable_on_ref (#a:Type) (#rel:preorder a) (r:mref a rel) (q : a -> prop) : Type =
   forall (v1 v2 : a). q v1 /\ rel v1 v2 ==> q v2
 
@@ -87,55 +105,50 @@ let witnessed_on_ref_prop (#a:Type) (#rel:preorder a) (r:mref a rel) (q : (a -> 
 let witnessed_on_ref (#a:Type) (#rel:preorder a) (r:mref a rel) (q : (a -> prop){stable_on_ref r q}) : Type =
   witnessed (witnessed_on_ref_prop r q)
 
-assume val witness: (#a:Type) -> (#rel:preorder a) -> (r:mref a rel) -> q:(a -> prop) -> ST unit
+val witness: (#a:Type) -> (#rel:preorder a) -> (r:mref a rel) -> q:(a -> prop) -> ST unit
     (requires (fun h -> h `contains` r /\ q (sel h r) /\ stable_on_ref r q
 				 /\ (witnessed_on_ref_prop r q h)
     
     ))
     (ensures (fun h0 _ h1 -> witnessed_on_ref r q /\ h0 == h1))
-//let witness #a #rel r q =
-//  gst_witness (witnessed_on_ref_prop r q)
+let witness #a #rel r q =
+  gst_witness (witnessed_on_ref_prop r q)
 
-assume val recall : (#a:Type) -> (#rel:preorder a) -> (r:mref a rel) -> q:(a -> prop) -> ST unit
+val recall : (#a:Type) -> (#rel:preorder a) -> (r:mref a rel) -> q:(a -> prop) -> ST unit
     (requires (fun h -> stable_on_ref r q /\ witnessed_on_ref r q /\ h `contains` r))
     (ensures (fun h0 _ h1 -> q (sel h1 r) /\ h0 == h1))
-//let recall #a #rel r q =
-  //gst_recall (witnessed_on_ref_prop r q)
+let recall #a #rel r q =
+  gst_recall (witnessed_on_ref_prop r q)
 
-//abstract let
-assume val
-alloc (#a:Type) (#rel:preorder a) (init:a)
+abstract let alloc (#a:Type) (#rel:preorder a) (init:a)
   :ST (mref a rel)
       (fun h -> True)
       (fun h0 r h1 -> fresh r h0 h1 /\ modifies Set.empty h0 h1 /\ sel h1 r == init)
-//  = let h0 = gst_get () in
-//    let r, h1 = alloc rel h0 init in
-//    gst_put h1;
-//    r
-
-//abstract let
-assume val read (#a:Type) (#rel:preorder a) (r:mref a rel) :STATE a (fun p h -> h `contains` r /\ p (sel h r) h)
-//  = let h0 = gst_get () in
-//    ManualHeap.lemma_sel_equals_sel_tot_for_contained_refs h0 r;
-//    sel_tot h0 r
+  = let h0 = gst_get () in
+    let r, h1 = alloc rel h0 init in
+    gst_put h1;
+    r
 
 
-//abstract let
-assume val write (#a:Type) (#rel:preorder a) (r:mref a rel) (v:a)
+abstract let read (#a:Type) (#rel:preorder a) (r:mref a rel) :STATE a (fun p h -> h `contains` r /\ p (sel h r) h)
+  = let h0 = gst_get () in
+    ManualHeap.lemma_sel_equals_sel_tot_for_contained_refs h0 r;
+    sel_tot h0 r
+
+
+abstract let write (#a:Type) (#rel:preorder a) (r:mref a rel) (v:a)
   : ST unit
-    (fun h -> rel (sel h r) v /\ h `contains` r)
+    (fun h -> rel (sel h r) v /\ h `contains` r /\ prefix (pos_of h) (fst (addr_of r)))
     (fun h0 x h1 -> rel (sel h0 r) v /\ h0 `contains` r /\
                  modifies (Set.singleton (addr_of r)) h0 h1 /\ equal_dom h0 h1 /\
                  sel h1 r == v)
-//  = let h0 = gst_get () in
-//    let h1 = upd_tot h0 r v in
-//    ManualHeap.lemma_distinct_addrs_distinct_preorders ();
-//    ManualHeap.lemma_upd_equals_upd_tot_for_contained_refs h0 r v;
-//    gst_put h1
+  = let h0 = gst_get () in
+    let h1 = upd_tot h0 r v in
+    ManualHeap.lemma_distinct_addrs_distinct_preorders ();
+    ManualHeap.lemma_upd_equals_upd_tot_for_contained_refs h0 r v;
+    gst_put h1
 
-//abstract let
-assume val get (u:unit) :ST heap (fun h -> True) (fun h0 h h1 -> h0==h1 /\ h==h1)
-//= gst_get ()
+abstract let get (u:unit) :ST heap (fun h -> True) (fun h0 h h1 -> h0==h1 /\ h==h1) = gst_get ()
 
 abstract
 let op_Bang (#a:Type) (#rel:preorder a) (r:mref a rel)
@@ -144,7 +157,7 @@ let op_Bang (#a:Type) (#rel:preorder a) (r:mref a rel)
 
 abstract let op_Colon_Equals (#a:Type) (#rel:preorder a) (r:mref a rel) (v:a)
   : ST unit
-    (fun h -> rel (sel h r) v /\ h `contains` r)
+    (fun h -> rel (sel h r) v /\ h `contains` r /\ prefix (pos_of h) (fst (addr_of r)))
     (fun h0 x h1 -> rel (sel h0 r) v /\ h0 `contains` r /\
                  modifies (Set.singleton (addr_of r)) h0 h1 /\ equal_dom h0 h1 /\
                  sel h1 r == v)
